src/lib/communication/DY.Lib.Communication.Core.Lemmas.fst
@@ -27,12 +27,12 @@ open DY.Lib.Communication.Core.Invariants
 
 [@@"opaque_to_smt"]
 val core_comm_layer_lemmas_enabled:
-  #a:Type -> {| parseable_serializeable bytes a |} ->
+  #a:Type -> {|comm_layer_core_config a|} ->
   comm_higher_layer_event_preds a -> prop
 let core_comm_layer_lemmas_enabled _ = True
 
 val enable_core_comm_layer_lemmas:
-  #a:Type -> {| parseable_serializeable bytes a |} ->
+  #a:Type -> {|comm_layer_core_config a|} ->
   preds:comm_higher_layer_event_preds a ->
   Lemma (core_comm_layer_lemmas_enabled preds)
 let enable_core_comm_layer_lemmas preds =
@@ -42,9 +42,9 @@ let enable_core_comm_layer_lemmas preds =
 
 #push-options "--ifuel 2"
 val initialize_communication_proof:
-  {|comm_layer_core_tag|} ->
   {|invs:protocol_invariants|} ->
   tr:trace ->
+  a:Type -> {|comm_layer_core_config a|} ->
   sender:principal -> receiver:principal ->
   Lemma
   (requires
@@ -53,45 +53,42 @@ val initialize_communication_proof:
     has_pki_invariant
   )
   (ensures (
-    let (_, tr_out) = initialize_communication sender receiver tr in
+    let (_, tr_out) = initialize_communication a sender receiver tr in
     trace_invariant tr_out
   ))
   [SMTPat (trace_invariant #invs tr);
-   SMTPat (initialize_communication sender receiver tr);
+   SMTPat (initialize_communication a sender receiver tr);
   ]
-let initialize_communication_proof tr sender receiver =
-  reveal_opaque (`%initialize_communication) (initialize_communication sender receiver)
+let initialize_communication_proof tr a sender receiver =
+  reveal_opaque (`%initialize_communication) (initialize_communication a sender receiver)
 #pop-options
 
 (**** Confidential Send and Receive Lemmas ****)
 
 val encrypt_message_proof:
-  {|comm_layer_core_tag|} ->
   {|cinvs:crypto_invariants|} ->
-  #a:Type -> {| parseable_serializeable bytes a |} ->
+  #a:Type -> {|comm_layer_core_config a|} ->
   tr:trace ->
   sender:principal -> receiver:principal ->
   pk_receiver:bytes -> nonce:bytes -> payload:a ->
   Lemma
   (requires (
-    let payload_bytes = serialize #bytes a payload in
-    has_communication_layer_crypto_predicates /\
+    has_communication_layer_crypto_predicates a /\
     is_secret (long_term_key_label sender) tr nonce /\
     nonce `has_usage tr` PkeNonce /\
-    is_public_key_for tr pk_receiver (LongTermPkeKey comm_layer_pkenc_tag) receiver /\
-    is_knowable_by (join (principal_label sender) (principal_label receiver)) tr payload_bytes /\
-    event_triggered tr sender (CommConfSendMsg sender receiver payload_bytes)
+    is_public_key_for tr pk_receiver (LongTermPkeKey (comm_layer_pkenc_tag a)) receiver /\
+    is_well_formed a (is_knowable_by (join (principal_label sender) (principal_label receiver)) tr) payload /\
+    event_triggered tr sender (CommConfSendMsg sender receiver payload <: communication_core_event a)
   ))
   (ensures
     is_publishable tr (encrypt_message pk_receiver nonce payload)
   )
-let encrypt_message_proof #tag #cinvs #a tr sender receiver pk_receiver nonce pkenc_in =
+let encrypt_message_proof #cinvs #a tr sender receiver pk_receiver nonce pkenc_in =
   reveal_opaque (`%encrypt_message) (encrypt_message #a)
 
 val send_confidential_proof:
-  {|comm_layer_core_tag|} ->
   {|invs:protocol_invariants|} ->
-  #a:Type -> {| parseable_serializeable bytes a |} ->
+  #a:Type0 -> {|comm_layer_core_config a|} ->
   tr:trace ->
   higher_layer_preds:comm_higher_layer_event_preds a ->
   keys_sess_ids:communication_keys_sess_ids ->
@@ -100,8 +97,8 @@ val send_confidential_proof:
   (requires (
     trace_invariant tr /\
     has_pki_invariant /\
-    has_communication_layer_crypto_predicates /\
-    has_communication_layer_event_predicates higher_layer_preds /\
+    has_communication_layer_crypto_predicates a /\
+    has_communication_layer_event_predicates a higher_layer_preds /\
     higher_layer_preds.send_conf tr sender receiver payload /\
     // We only require the payload to flow to the sender and receiver to allow
     // the sender to send a payload readable by other principals. If you want
@@ -117,17 +114,15 @@ val send_confidential_proof:
   [SMTPat (trace_invariant #invs tr);
    SMTPat (send_confidential keys_sess_ids sender receiver payload tr);
    SMTPat (core_comm_layer_lemmas_enabled higher_layer_preds)]
-let send_confidential_proof #tag #invs #a tr higher_layer_preds keys_sess_ids sender receiver payload =
-  reveal_opaque (`%send_confidential) (send_confidential #tag #a);
+let send_confidential_proof #invs #a tr higher_layer_preds keys_sess_ids sender receiver payload =
+  reveal_opaque (`%send_confidential) (send_confidential #a);
   match send_confidential keys_sess_ids sender receiver payload tr with
   | (None, tr_out) -> ()
   | (Some _, tr_out) -> (
-    let (Some pk_receiver, tr') = get_public_key sender keys_sess_ids.pki (LongTermPkeKey comm_layer_pkenc_tag) receiver tr in
+    let (Some pk_receiver, tr') = get_public_key sender keys_sess_ids.pki (LongTermPkeKey (comm_layer_pkenc_tag a)) receiver tr in
     let (nonce, tr') = mk_rand PkeNonce (long_term_key_label sender) 32 tr' in
-    let payload_bytes = serialize #bytes a payload in
-    assert(is_knowable_by (comm_label sender receiver) tr payload_bytes);
     higher_layer_preds.send_conf_later tr tr' sender receiver payload;
-    let ((), tr') = trigger_event sender (CommConfSendMsg sender receiver payload_bytes) tr' in
+    let ((), tr') = trigger_event sender (CommConfSendMsg sender receiver payload <: communication_core_event a) tr' in
     encrypt_message_proof tr' sender receiver pk_receiver nonce payload;
     let msg_encrypted = encrypt_message pk_receiver nonce payload in
     let (msg_id, tr') = send_msg msg_encrypted tr' in
@@ -136,15 +131,14 @@ let send_confidential_proof #tag #invs #a tr higher_layer_preds keys_sess_ids se
   )
 
 val decrypt_message_proof:
-  {|comm_layer_core_tag|} ->
   {|cinvs:crypto_invariants|} ->
-  #a:Type -> {| parseable_serializeable bytes a |} ->
+  #a:Type0 -> {|comm_layer_core_config a|} ->
   tr:trace ->
   receiver:principal -> sk_receiver:bytes -> msg_encrypted:bytes ->
   Lemma
   (requires
-    has_communication_layer_crypto_predicates /\
-    is_private_key_for tr sk_receiver (LongTermPkeKey comm_layer_pkenc_tag) receiver /\
+    has_communication_layer_crypto_predicates a /\
+    is_private_key_for tr sk_receiver (LongTermPkeKey (comm_layer_pkenc_tag a)) receiver /\
     bytes_invariant tr msg_encrypted
   )
   (ensures
@@ -153,15 +147,15 @@ val decrypt_message_proof:
       | None -> True
       | Some payload -> (exists sender.
         is_well_formed a (is_knowable_by (comm_label sender receiver) tr) payload /\
-        is_knowable_by (comm_label sender receiver) tr (serialize a payload) /\
+        is_well_formed a (is_knowable_by (comm_label sender receiver) tr) payload /\
         (
-          event_triggered tr sender (CommConfSendMsg sender receiver (serialize a payload)) \/
+          event_triggered tr sender (CommConfSendMsg sender receiver payload <: communication_core_event a) \/
           is_well_formed a (is_publishable tr) payload
         )
       )
     )
   )
-let decrypt_message_proof #tag #cinvs #a tr receiver sk_receiver msg_encrypted =
+let decrypt_message_proof #cinvs #a tr receiver sk_receiver msg_encrypted =
   reveal_opaque (`%decrypt_message) (decrypt_message #a);
   match decrypt_message #a sk_receiver msg_encrypted with
   | None -> ()
@@ -172,9 +166,8 @@ let decrypt_message_proof #tag #cinvs #a tr receiver sk_receiver msg_encrypted =
   )
 
 val receive_confidential_proof:
-  {|tag:comm_layer_core_tag|} ->
   {|invs:protocol_invariants|} ->
-  #a:Type -> {| parseable_serializeable bytes a |} ->
+  #a:Type0 -> {|comm_layer_core_config a|} ->
   tr:trace ->
   higher_layer_preds:comm_higher_layer_event_preds a ->
   comm_keys_ids:communication_keys_sess_ids ->
@@ -183,30 +176,30 @@ val receive_confidential_proof:
   (requires
     trace_invariant tr /\
     has_private_keys_invariant /\
-    has_communication_layer_crypto_predicates /\
-    has_communication_layer_event_predicates higher_layer_preds
+    has_communication_layer_crypto_predicates a /\
+    has_communication_layer_event_predicates a higher_layer_preds
   )
   (ensures (
     match receive_confidential comm_keys_ids receiver msg_id tr with
     | (None, tr_out) -> trace_invariant tr_out
     | (Some payload, tr_out) ->
       trace_invariant tr_out /\
-      event_triggered tr_out receiver (CommConfReceiveMsg receiver (serialize a payload)) /\
+      event_triggered tr_out receiver (CommConfReceiveMsg receiver payload <: communication_core_event a) /\
       is_well_formed a (is_knowable_by (principal_label receiver) tr) payload
   ))
   [SMTPat (trace_invariant tr);
-   SMTPat (receive_confidential #tag #a comm_keys_ids receiver msg_id tr);
+   SMTPat (receive_confidential #a comm_keys_ids receiver msg_id tr);
    SMTPat (core_comm_layer_lemmas_enabled higher_layer_preds)]
-let receive_confidential_proof #tag #invs #a tr higher_layer_preds comm_keys_ids receiver msg_id =
-  reveal_opaque (`%receive_confidential) (receive_confidential #tag #a);
+let receive_confidential_proof #invs #a tr higher_layer_preds comm_keys_ids receiver msg_id =
+  reveal_opaque (`%receive_confidential) (receive_confidential #a);
   match receive_confidential comm_keys_ids receiver msg_id tr with
   | (None, tr_out) -> ()
   | (Some payload, tr_out) -> (
-    let (Some sk_receiver, tr) = get_private_key receiver comm_keys_ids.private_keys (LongTermPkeKey comm_layer_pkenc_tag) tr in
+    let (Some sk_receiver, tr) = get_private_key receiver comm_keys_ids.private_keys (LongTermPkeKey (comm_layer_pkenc_tag a)) tr in
     let (Some msg_encrypted, tr) = recv_msg msg_id tr in
-    decrypt_message_proof #tag #invs.crypto_invs #a tr receiver sk_receiver msg_encrypted;
+    decrypt_message_proof #invs.crypto_invs #a tr receiver sk_receiver msg_encrypted;
     let Some msg_plain = decrypt_message #a sk_receiver msg_encrypted in
-    let ((), tr) = trigger_event receiver (CommConfReceiveMsg receiver (serialize a payload)) tr in
+    let ((), tr) = trigger_event receiver (CommConfReceiveMsg receiver payload <: communication_core_event a) tr in
     assert(tr_out == tr);
     assert(trace_invariant tr_out);
     ()
@@ -216,58 +209,57 @@ let receive_confidential_proof #tag #invs #a tr higher_layer_preds comm_keys_ids
 (**** Authenticated Send and Receive Lemmas ****)
 
 val sign_message_proof:
-  {|comm_layer_core_tag|} ->
   {|cinvs:crypto_invariants|} ->
-  #a:Type -> {| parseable_serializeable bytes a |} ->
+  #a:Type0 -> {|config:comm_layer_core_config a|} ->
   tr:trace ->
-  sender:principal -> receiver:principal -> payload:a -> pk_receiver:option bytes ->
+  sender:principal -> receiver:principal -> payload:either a bytes -> pk_receiver:option bytes ->
   sk_sender:bytes -> nonce:bytes ->
   Lemma
   (requires (
-    let payload_bytes = serialize a payload in
-    has_communication_layer_crypto_predicates /\
+    (Some? pk_receiver <==> Inr? payload) /\ 
+    (None? pk_receiver <==> Inl? payload) /\
+    has_communication_layer_crypto_predicates a /\
     is_secret (long_term_key_label sender) tr nonce /\
     nonce `has_usage tr` SigNonce /\
-    is_private_key_for tr sk_sender (LongTermSigKey comm_layer_sign_tag) sender /\
-    is_well_formed a (is_publishable tr) payload /\
+    is_private_key_for tr sk_sender (LongTermSigKey (comm_layer_sign_tag a)) sender /\
     (
       match pk_receiver with
-      | None -> event_triggered tr sender (CommAuthSendMsg sender payload_bytes)
+      | None -> (
+        is_well_formed a (is_publishable tr) (Inl?.v payload) /\
+        event_triggered tr sender (CommAuthSendMsg sender (Inl?.v payload) <: communication_core_event a)
+      )
       | Some pk -> (
-        match parse com_send_byte payload_bytes with
-        | None -> False
-        | Some payload ->
-          (exists plain_payload nonce.
-            is_publishable tr pk /\
-            payload.b == pke_enc pk nonce plain_payload /\
-            event_triggered tr sender (CommConfAuthSendMsg sender receiver plain_payload)
-          )
+        is_publishable tr (Inr?.v payload) /\
+        is_publishable tr pk /\
+        (exists plain_payload nonce.
+          Inr?.v payload == pke_enc pk nonce plain_payload /\
+          (match parse a #(parseable_serializeable_bytes_a #a) plain_payload with
+          | None -> False
+          | Some plain_payload_parsed -> event_triggered tr sender (CommConfAuthSendMsg sender receiver plain_payload_parsed <: communication_core_event a))
+        )
       )
     )
   ))
   (ensures
     is_publishable tr (sign_message sender receiver payload pk_receiver sk_sender nonce)
   )
-let sign_message_proof #tag #cinvs #a tr sender receiver payload pk_receiver sk_sender nonce =
+let sign_message_proof #cinvs #a #config tr sender receiver payload pk_receiver sk_sender nonce =
   reveal_opaque (`%sign_message) (sign_message #a);
-  let payload_bytes = serialize a payload in
-  assert(is_publishable tr payload_bytes);
   let sig_input = match pk_receiver with
-    | None -> Plain sender receiver payload_bytes
-    | Some pk -> Encrypted sender receiver payload_bytes pk
-  in
+    | None -> Plain sender receiver (serialize a (Inl?.v payload))
+    | Some pk -> Encrypted sender receiver (Inr?.v payload) pk
+  in 
   let sig_input_bytes = serialize signature_input sig_input in
   serialize_wf_lemma signature_input (is_publishable tr) sig_input;
   let signature = sign sk_sender nonce sig_input_bytes in
   let msg_signed = SigMessage {msg=sig_input_bytes; signature} in
   assert(bytes_invariant tr signature);
-  serialize_wf_lemma com_message_t (is_publishable tr) msg_signed;
+  serialize_wf_lemma comm_message_t (is_publishable tr) msg_signed;
   ()
 
 val send_authenticated_proof:
-  {|event_tag:comm_layer_core_tag|} ->
   {|invs:protocol_invariants|} ->
-  #a:Type -> {| parseable_serializeable bytes a |} ->
+  #a:Type -> {|comm_layer_core_config a|} ->
   tr:trace ->
   higher_layer_preds:comm_higher_layer_event_preds a ->
   comm_keys_ids:communication_keys_sess_ids ->
@@ -276,8 +268,8 @@ val send_authenticated_proof:
   (requires
     trace_invariant tr /\
     has_private_keys_invariant /\
-    has_communication_layer_crypto_predicates /\
-    has_communication_layer_event_predicates higher_layer_preds /\
+    has_communication_layer_crypto_predicates a /\
+    has_communication_layer_event_predicates a higher_layer_preds /\
     higher_layer_preds.send_auth tr sender payload /\
     is_well_formed a (is_publishable tr) payload
   )
@@ -288,19 +280,18 @@ val send_authenticated_proof:
   [SMTPat (trace_invariant #invs tr);
    SMTPat (send_authenticated comm_keys_ids sender receiver payload tr);
    SMTPat (core_comm_layer_lemmas_enabled higher_layer_preds)]
-let send_authenticated_proof #tag #invs #a tr higher_layer_preds comm_keys_ids sender receiver payload =
-    reveal_opaque (`%send_authenticated) (send_authenticated #tag #a);
+let send_authenticated_proof #invs #a tr higher_layer_preds comm_keys_ids sender receiver payload =
+    reveal_opaque (`%send_authenticated) (send_authenticated #a);
     match send_authenticated comm_keys_ids sender receiver payload tr with
     | (None, tr_out) -> ()
     | (Some _, tr_out) -> (
-      let (Some sk_sender, tr') = get_private_key sender comm_keys_ids.private_keys (LongTermSigKey comm_layer_sign_tag) tr in
+      let (Some sk_sender, tr') = get_private_key sender comm_keys_ids.private_keys (LongTermSigKey (comm_layer_sign_tag a)) tr in
       let (nonce,  tr') = mk_rand SigNonce (long_term_key_label sender) 32 tr' in
       higher_layer_preds.send_auth_later tr tr' sender payload;
-      let payload_bytes = serialize a payload in
-      let ((), tr') = trigger_event sender (CommAuthSendMsg sender payload_bytes) tr' in
-      assert(event_triggered tr' sender (CommAuthSendMsg sender payload_bytes));
-      sign_message_proof #tag #invs.crypto_invs #a tr' sender receiver payload None sk_sender nonce;
-      let msg_signed = sign_message #a sender receiver payload None sk_sender nonce in
+      let ((), tr') = trigger_event sender (CommAuthSendMsg sender payload <: communication_core_event a) tr' in
+      assert(event_triggered tr' sender (CommAuthSendMsg sender payload <: communication_core_event a));
+      sign_message_proof #invs.crypto_invs #a tr' sender receiver (Inl payload) None sk_sender nonce;
+      let msg_signed = sign_message #a sender receiver (Inl payload) None sk_sender nonce in
       let (msg_id, tr') = send_msg msg_signed tr' in
       assert(tr_out == tr');
       assert(trace_invariant tr_out);
@@ -308,82 +299,75 @@ let send_authenticated_proof #tag #invs #a tr higher_layer_preds comm_keys_ids s
     )
 
 
-#push-options "--z3rlimit 50"
 val verify_message_proof:
-  {|comm_layer_core_tag|} ->
   {|cinvs:crypto_invariants|} ->
-  #a:Type -> {| ps:parseable_serializeable bytes a |} ->
+  #a:Type -> {|config:comm_layer_core_config a|} ->
   tr:trace ->
   sender:principal -> receiver:principal ->
   msg_bytes:bytes -> sk_receiver_opt:option bytes ->
   vk_sender:bytes ->
   Lemma
   (requires
-    has_communication_layer_crypto_predicates /\
+    has_communication_layer_crypto_predicates a /\
     is_publishable tr msg_bytes /\
-    is_public_key_for tr vk_sender (LongTermSigKey comm_layer_sign_tag) sender
+    is_public_key_for tr vk_sender (LongTermSigKey (comm_layer_sign_tag a)) sender
   )
   (ensures (
     match verify_message #a receiver msg_bytes sk_receiver_opt vk_sender with
-    | Some cm -> (
-      let Some msg_signed_t = parse com_message_t msg_bytes in
+    | Some payload -> (
+      let Some msg_signed_t = parse comm_message_t msg_bytes in
       let SigMessage msg_signed = msg_signed_t in
-      let Some sign_input = parse signature_input #parseable_serializeable_bytes_signature_input msg_signed.msg in
-      let payload_bytes = serialize a cm.payload in
-      is_well_formed a (is_publishable tr) cm.payload /\
+      let Some sign_input = parse signature_input msg_signed.msg in
       (
-        (
-          cm.sender == sender /\
-          cm.receiver == receiver /\
-          (match sign_input with
-            | Plain sender' receiver' payload_bytes' -> (
-              event_triggered tr sender (CommAuthSendMsg sender payload_bytes)
-            )
-            | Encrypted sender' receiver' payload_bytes' pk_receiver -> (
-              match parse com_send_byte payload_bytes with
-              | None -> True
-              | Some payload -> (
-                exists plain_payload nonce.
-                  payload.b == pke_enc pk_receiver nonce plain_payload /\
-                  event_triggered tr sender (CommConfAuthSendMsg sender receiver plain_payload)
-                )
+        match sign_input with
+        | Plain sender' receiver' payload_bytes' -> (
+          is_well_formed a (is_publishable tr) (Inl?.v payload) /\
+          (
+            event_triggered tr sender (CommAuthSendMsg sender (Inl?.v payload) <: communication_core_event a) \/ 
+            is_corrupt tr (long_term_key_label sender)
+          )
+        )
+        | Encrypted sender' receiver' payload_bytes' pk_receiver -> (
+          is_publishable tr (Inr?.v payload) /\
+          (
+            (
+              exists plain_payload nonce.
+                (Inr?.v payload) == pke_enc pk_receiver nonce plain_payload /\
+                (match parse a plain_payload with
+                | None -> False
+                | Some plain_payload_parsed -> event_triggered tr sender (CommConfAuthSendMsg sender receiver plain_payload_parsed <: communication_core_event a))
+            ) \/ (
+              is_corrupt tr (long_term_key_label sender)
             )
           )
-        ) \/ (
-          is_corrupt tr (long_term_key_label sender)
         )
       )
     )
     | _ -> True
   ))
-let verify_message_proof #tag #cinvs #a #ps tr sender receiver msg_bytes sk_receiver_opt vk_sender =
+let verify_message_proof #cinvs #a #config tr sender receiver msg_bytes sk_receiver_opt vk_sender =
   assert(get_signkey_label tr vk_sender == long_term_key_label sender);
   match verify_message #a receiver msg_bytes sk_receiver_opt vk_sender with
   | None -> ()
-  | Some cm -> (
-    parse_wf_lemma com_message_t (is_publishable tr) msg_bytes;
-    let Some msg_signed_t = parse com_message_t msg_bytes in
+  | Some payload -> (
+    parse_wf_lemma comm_message_t (is_publishable tr) msg_bytes;
+    let Some msg_signed_t = parse comm_message_t msg_bytes in
     let SigMessage msg_signed = msg_signed_t in
-    parse_wf_lemma signature_input #parseable_serializeable_bytes_signature_input (is_publishable tr) msg_signed.msg;
-    let Some sign_input = parse signature_input #parseable_serializeable_bytes_signature_input msg_signed.msg in
-
+    parse_wf_lemma signature_input (is_publishable tr) msg_signed.msg;
+    let Some sign_input = parse signature_input msg_signed.msg in
     match sign_input with
     | Plain sender' receiver' payload_bytes' -> (
-      serialize_parse_inv_lemma #bytes a #ps payload_bytes';
+      serialize_parse_inv_lemma a payload_bytes';
       ()
     )
     | Encrypted sender' receiver' payload_bytes' pk_receiver -> (
-      serialize_parse_inv_lemma #bytes a #ps payload_bytes';
-      assert(payload_bytes' == serialize a cm.payload);
       ()
     )
   )
-#pop-options
 
 val receive_authenticated_proof:
-  {|tag:comm_layer_core_tag|} ->
   {|invs:protocol_invariants|} ->
-  #a:Type -> {| parseable_serializeable bytes a |} ->
+  #a:Type -> {|config:comm_layer_core_config a|} ->
   tr:trace ->
   higher_layer_preds:comm_higher_layer_event_preds a ->
   comm_keys_ids:communication_keys_sess_ids ->
@@ -392,76 +376,76 @@ val receive_authenticated_proof:
   (requires
     trace_invariant tr /\
     has_pki_invariant /\
-    has_communication_layer_crypto_predicates /\
-    has_communication_layer_event_predicates higher_layer_preds
+    has_communication_layer_crypto_predicates a /\
+    has_communication_layer_event_predicates a higher_layer_preds
   )
   (ensures (
     match receive_authenticated comm_keys_ids receiver msg_id tr with
     | (None, tr_out) -> trace_invariant tr_out
     | (Some cm, tr_out) -> (
       trace_invariant tr_out /\
-      event_triggered tr_out receiver (CommAuthReceiveMsg cm.sender receiver (serialize a cm.payload)) /\
+      event_triggered tr_out receiver (CommAuthReceiveMsg cm.sender receiver cm.payload <: communication_core_event a) /\
       is_well_formed a (is_publishable tr) cm.payload
     )
   ))
   [SMTPat (trace_invariant #invs tr);
-   SMTPat (receive_authenticated #tag #a comm_keys_ids receiver msg_id tr);
+   SMTPat (receive_authenticated #a comm_keys_ids receiver msg_id tr);
    SMTPat (core_comm_layer_lemmas_enabled higher_layer_preds)]
-let receive_authenticated_proof #tag #invs #a tr higher_layer_preds comm_keys_ids receiver msg_id =
-  reveal_opaque (`%receive_authenticated) (receive_authenticated #tag #a);
-  match receive_authenticated #tag #a comm_keys_ids receiver msg_id tr with
+let receive_authenticated_proof #invs #a tr higher_layer_preds comm_keys_ids receiver msg_id =
+  reveal_opaque (`%receive_authenticated) (receive_authenticated #a);
+  match receive_authenticated #a comm_keys_ids receiver msg_id tr with
   | (None, tr_out) -> ()
   | (Some cm', tr_out) -> (
     let (Some msg_signed_bytes, tr) = recv_msg msg_id tr in
     let Some sender = get_sender msg_signed_bytes in
-    let (Some vk_sender, tr) = get_public_key receiver comm_keys_ids.pki (LongTermSigKey comm_layer_sign_tag) sender tr in
-    verify_message_proof #tag #invs.crypto_invs #a tr sender receiver msg_signed_bytes None vk_sender;
-    let (Some cm) = verify_message #a receiver msg_signed_bytes None vk_sender in
-    let ((), tr) = trigger_event receiver (CommAuthReceiveMsg sender receiver (serialize a cm.payload)) tr in
-    assert(tr_out == tr);
-    assert(trace_invariant tr_out);
+    let (Some vk_sender, tr) = get_public_key receiver comm_keys_ids.pki (LongTermSigKey (comm_layer_sign_tag a)) sender tr in
+    verify_message_proof #invs.crypto_invs #a tr sender receiver msg_signed_bytes None vk_sender;
+    match verify_message #a receiver msg_signed_bytes None vk_sender with
+    | None -> ()
+    | Some (Inl payload) -> (
+      let ((), tr) = trigger_event receiver (CommAuthReceiveMsg sender receiver payload <: communication_core_event a) tr in
+      assert(tr_out == tr);
+      assert(trace_invariant tr_out);
     ()
+    )
   )
 
 
 (**** Confidential and Authenticates Send and Receive Lemmas ****)
 
 val encrypt_and_sign_message_proof:
-  {|comm_layer_core_tag|} ->
   {|cinvs:crypto_invariants|} ->
-  #a:Type -> {| parseable_serializeable bytes a |} ->
+  #a:Type -> {|comm_layer_core_config a|} ->
   tr:trace ->
   sender:principal -> receiver:principal -> payload:a ->
   pk_receiver:bytes -> sk_sender:bytes -> enc_nonce:bytes -> sign_nonce:bytes ->
   Lemma
-  (requires (
-    let payload_bytes = serialize #bytes a payload in
-    has_communication_layer_crypto_predicates /\
+  (requires
+    has_communication_layer_crypto_predicates a /\
     is_secret (long_term_key_label sender) tr enc_nonce /\
     is_secret (long_term_key_label sender) tr sign_nonce /\
     enc_nonce `has_usage tr` PkeNonce /\
     sign_nonce `has_usage tr` SigNonce /\
-    is_public_key_for tr pk_receiver (LongTermPkeKey comm_layer_pkenc_tag) receiver /\
-    is_private_key_for tr sk_sender (LongTermSigKey comm_layer_sign_tag) sender /\
-    is_knowable_by (join (principal_label sender) (principal_label receiver)) tr payload_bytes /\
-    event_triggered tr sender (CommConfSendMsg sender receiver payload_bytes) /\
-    event_triggered tr sender (CommConfAuthSendMsg sender receiver payload_bytes)
-  ))
+    is_public_key_for tr pk_receiver (LongTermPkeKey (comm_layer_pkenc_tag a)) receiver /\
+    is_private_key_for tr sk_sender (LongTermSigKey (comm_layer_sign_tag a)) sender /\
+    is_well_formed a (is_knowable_by (comm_label sender receiver) tr) payload /\
+    event_triggered tr sender (CommConfSendMsg sender receiver payload <: communication_core_event a) /\
+    event_triggered tr sender (CommConfAuthSendMsg sender receiver payload <: communication_core_event a)
+  )
   (ensures
     is_publishable tr (encrypt_and_sign_message sender receiver payload pk_receiver sk_sender enc_nonce sign_nonce)
   )
-let encrypt_and_sign_message_proof #tag #cinvs #a tr sender receiver payload pk_receiver sk_sender enc_nonce sign_nonce =
+let encrypt_and_sign_message_proof #cinvs #a tr sender receiver payload pk_receiver sk_sender enc_nonce sign_nonce =
   reveal_opaque (`%encrypt_and_sign_message) (encrypt_and_sign_message #a);
   reveal_opaque (`%encrypt_message) (encrypt_message #a); // TODO: This should be removeable.
   encrypt_message_proof tr sender receiver pk_receiver enc_nonce payload;
   let enc_payload = encrypt_message pk_receiver enc_nonce payload in
-  sign_message_proof tr sender receiver {b=enc_payload} (Some pk_receiver) sk_sender sign_nonce;
+  sign_message_proof #cinvs #a tr sender receiver (Inr enc_payload) (Some pk_receiver) sk_sender sign_nonce;
   ()
 
 val send_confidential_authenticated_proof:
-  {|tag:comm_layer_core_tag|} ->
-  {|invs:protocol_invariants|} ->
-  #a:Type -> {| parseable_serializeable bytes a |} ->
+  {|protocol_invariants|} ->
+  #a:Type0 -> {|comm_layer_core_config a|}  ->
   tr:trace ->
   higher_layer_preds:comm_higher_layer_event_preds a ->
   comm_keys_ids:communication_keys_sess_ids ->
@@ -471,8 +455,8 @@ val send_confidential_authenticated_proof:
     trace_invariant tr /\
     has_private_keys_invariant /\
     has_pki_invariant /\
-    has_communication_layer_crypto_predicates /\
-    has_communication_layer_event_predicates higher_layer_preds /\
+    has_communication_layer_crypto_predicates a /\
+    has_communication_layer_event_predicates a higher_layer_preds /\
     higher_layer_preds.send_conf tr sender receiver payload /\
     higher_layer_preds.send_conf_auth tr sender receiver payload /\
     is_well_formed a (is_knowable_by (join (principal_label sender) (principal_label receiver)) tr) payload
@@ -481,27 +465,27 @@ val send_confidential_authenticated_proof:
     let (_, tr_out) = send_confidential_authenticated comm_keys_ids sender receiver payload tr in
     trace_invariant tr_out
   ))
-  [SMTPat (trace_invariant #invs tr);
-   SMTPat (send_confidential_authenticated #tag #a comm_keys_ids sender receiver payload tr);
+  [SMTPat (trace_invariant tr);
+   SMTPat (send_confidential_authenticated comm_keys_ids sender receiver payload tr);
    SMTPat (core_comm_layer_lemmas_enabled higher_layer_preds)]
-let send_confidential_authenticated_proof #tag #invs #a tr higher_layer_preds comm_keys_ids sender receiver payload =
-  reveal_opaque (`%send_confidential_authenticated) (send_confidential_authenticated #tag #a);
+let send_confidential_authenticated_proof #invs #a tr higher_layer_preds comm_keys_ids sender receiver payload =
+  reveal_opaque (`%send_confidential_authenticated) (send_confidential_authenticated #a);
   match send_confidential_authenticated comm_keys_ids sender receiver payload tr with
   | (None, tr_out) -> ()
   | (Some _, tr_out) -> (
-    let (Some pk_receiver, tr') = get_public_key sender comm_keys_ids.pki (LongTermPkeKey comm_layer_pkenc_tag) receiver tr in
-    let (Some sk_sender, tr') = get_private_key  sender comm_keys_ids.private_keys (LongTermSigKey comm_layer_sign_tag) tr' in
+    let (Some pk_receiver, tr') = get_public_key sender comm_keys_ids.pki (LongTermPkeKey (comm_layer_pkenc_tag a)) receiver tr in
+    let (Some sk_sender, tr') = get_private_key  sender comm_keys_ids.private_keys (LongTermSigKey (comm_layer_sign_tag a)) tr' in
     let (enc_nonce, tr') = mk_rand PkeNonce (long_term_key_label sender) 32 tr' in
     let (sign_nonce, tr') = mk_rand SigNonce (long_term_key_label sender) 32 tr' in
 
     let payload_bytes = serialize #bytes a payload in
     higher_layer_preds.send_conf_later tr tr' sender receiver payload;
-    let ((), tr') = trigger_event sender (CommConfSendMsg sender receiver payload_bytes) tr' in
-    assert(event_triggered tr' sender (CommConfSendMsg sender receiver payload_bytes));
+    let ((), tr') = trigger_event sender (CommConfSendMsg sender receiver payload <: communication_core_event a) tr' in
+    assert(event_triggered tr' sender (CommConfSendMsg sender receiver payload <: communication_core_event a));
 
     higher_layer_preds.send_conf_auth_later tr tr' sender receiver payload;
-    let ((), tr') = trigger_event sender (CommConfAuthSendMsg sender receiver payload_bytes) tr' in
-    assert(event_triggered tr' sender (CommConfAuthSendMsg sender receiver payload_bytes));
+    let ((), tr') = trigger_event sender (CommConfAuthSendMsg sender receiver payload <: communication_core_event a) tr' in
+    assert(event_triggered tr' sender (CommConfAuthSendMsg sender receiver payload <: communication_core_event a));
 
     encrypt_and_sign_message_proof tr' sender receiver payload pk_receiver sk_sender enc_nonce sign_nonce;
     let msg = encrypt_and_sign_message sender receiver payload pk_receiver sk_sender enc_nonce sign_nonce in
@@ -514,57 +498,56 @@ let send_confidential_authenticated_proof #tag #invs #a tr higher_layer_preds co
 
 #push-options "--ifuel 1 --z3rlimit 40"
 val verify_and_decrypt_message_proof:
-  {|comm_layer_core_tag|} ->
   {|cinvs:crypto_invariants|} ->
-  #a:Type -> {| parseable_serializeable bytes a |} ->
+  #a:Type -> {|comm_layer_core_config a|} ->
   tr:trace ->
   sender:principal -> receiver:principal -> msg_encrypted_signed:bytes ->
   sk_receiver:bytes -> vk_sender:bytes ->
   Lemma
   (requires
-    has_communication_layer_crypto_predicates /\
+    has_communication_layer_crypto_predicates a /\
     is_publishable tr msg_encrypted_signed /\
-    is_private_key_for tr sk_receiver (LongTermPkeKey comm_layer_pkenc_tag) receiver /\
-    is_public_key_for tr vk_sender (LongTermSigKey comm_layer_sign_tag) sender
+    is_private_key_for tr sk_receiver (LongTermPkeKey (comm_layer_pkenc_tag a)) receiver /\
+    is_public_key_for tr vk_sender (LongTermSigKey (comm_layer_sign_tag a)) sender
   )
   (ensures (
     match verify_and_decrypt_message #a receiver sk_receiver vk_sender msg_encrypted_signed with
     | None -> True
     | Some cm -> (
       is_well_formed a (is_knowable_by (principal_label receiver) tr) cm.payload /\
-      is_knowable_by (principal_label receiver) tr (serialize a cm.payload) /\
+      //is_knowable_by (principal_label receiver) tr (serialize a cm.payload) /\
       (
-        event_triggered tr sender (CommConfAuthSendMsg sender receiver (serialize a cm.payload)) \/
+        event_triggered tr sender (CommConfAuthSendMsg sender receiver cm.payload <: communication_core_event a) \/
         is_corrupt tr (long_term_key_label sender)
       )
     )
   ))
-let verify_and_decrypt_message_proof #tag #cinvs #a tr sender receiver msg_encrypted_signed sk_receiver vk_sender =
+let verify_and_decrypt_message_proof #cinvs #a tr sender receiver msg_encrypted_signed sk_receiver vk_sender =
   reveal_opaque (`%verify_and_decrypt_message) (verify_and_decrypt_message #a);
   reveal_opaque (`%decrypt_message) (decrypt_message #a);
   match verify_and_decrypt_message #a receiver sk_receiver vk_sender msg_encrypted_signed with
   | None -> ()
   | Some cm -> (
-    verify_message_proof #tag #cinvs #com_send_byte tr sender receiver msg_encrypted_signed (Some sk_receiver) vk_sender;
-    let Some cm' = verify_message #com_send_byte receiver msg_encrypted_signed (Some sk_receiver) vk_sender in
-
-    let Some msg_signed_t = parse com_message_t msg_encrypted_signed in
+    verify_message_proof #cinvs #a tr sender receiver msg_encrypted_signed (Some sk_receiver) vk_sender;
+    let Some (Inr payload_enc) = verify_message #a receiver msg_encrypted_signed (Some sk_receiver) vk_sender in
+    let Some msg_signed_t = parse comm_message_t msg_encrypted_signed in
     let SigMessage msg_signed = msg_signed_t in
     let Some sign_input = parse signature_input msg_signed.msg in
     let Encrypted _ _ _ pk_receiver = sign_input in
     assert(pk_receiver == pk sk_receiver);
 
-    let Some plaintext = pke_dec sk_receiver cm'.payload.b in
+    let Some plaintext = pke_dec sk_receiver payload_enc in
     serialize_parse_inv_lemma #bytes a plaintext;
 
     introduce (~(is_corrupt tr (long_term_key_label sender))) ==>  (
-        event_triggered tr sender (CommConfAuthSendMsg sender receiver (serialize a cm.payload))
+        event_triggered tr sender (CommConfAuthSendMsg sender receiver cm.payload <: communication_core_event a)
       )
     with _. (
       eliminate exists plain_payload nonce.
-          cm'.payload.b == pke_enc pk_receiver nonce plain_payload /\
-          event_triggered tr sender (CommConfAuthSendMsg sender receiver plain_payload)
-      returns event_triggered tr sender (CommConfAuthSendMsg sender receiver (serialize a cm.payload))
+          payload_enc == pke_enc pk_receiver nonce plain_payload /\
+          Some? (parse a plain_payload) /\
+          event_triggered tr sender (CommConfAuthSendMsg sender receiver (Some?.v (parse a plain_payload)) <: communication_core_event a)
+      returns event_triggered tr sender (CommConfAuthSendMsg sender receiver cm.payload <: communication_core_event a)
       with _. (
         pke_dec_enc sk_receiver nonce plain_payload;
         ()
@@ -574,9 +557,8 @@ let verify_and_decrypt_message_proof #tag #cinvs #a tr sender receiver msg_encry
 #pop-options
 
 val receive_confidential_authenticated_proof:
-  {|tag:comm_layer_core_tag|} ->
   {|invs:protocol_invariants|} ->
-  #a:Type -> {| parseable_serializeable bytes a |} ->
+  #a:Type -> {|comm_layer_core_config a|} ->
   tr:trace ->
   higher_layer_preds:comm_higher_layer_event_preds a ->
   comm_keys_ids:communication_keys_sess_ids ->
@@ -586,37 +568,37 @@ val receive_confidential_authenticated_proof:
     trace_invariant tr /\
     has_private_keys_invariant /\
     has_pki_invariant /\
-    has_communication_layer_crypto_predicates /\
-    has_communication_layer_event_predicates higher_layer_preds
+    has_communication_layer_crypto_predicates a /\
+    has_communication_layer_event_predicates a higher_layer_preds
   )
   (ensures
     (
-      match receive_confidential_authenticated #tag #a comm_keys_ids receiver msg_id tr with
+      match receive_confidential_authenticated #a comm_keys_ids receiver msg_id tr with
       | (None, tr_out) -> trace_invariant tr_out
       | (Some cm, tr_out) -> (
         trace_invariant tr_out /\
-        event_triggered tr_out receiver (CommConfAuthReceiveMsg cm.sender receiver (serialize a cm.payload)) /\
+        event_triggered tr_out receiver (CommConfAuthReceiveMsg cm.sender receiver cm.payload <: communication_core_event a) /\
         is_well_formed a (is_knowable_by (principal_label receiver) tr) cm.payload
       )
     )
   )
   [SMTPat (trace_invariant #invs tr);
-   SMTPat (receive_confidential_authenticated #tag #a comm_keys_ids receiver msg_id tr);
+   SMTPat (receive_confidential_authenticated #a comm_keys_ids receiver msg_id tr);
    SMTPat (core_comm_layer_lemmas_enabled higher_layer_preds)]
-let receive_confidential_authenticated_proof #tag #invs #a tr higher_layer_preds comm_keys_ids receiver msg_id =
-  reveal_opaque (`%receive_confidential_authenticated) (receive_confidential_authenticated #tag #a);
+let receive_confidential_authenticated_proof #invs #a tr higher_layer_preds comm_keys_ids receiver msg_id =
+  reveal_opaque (`%receive_confidential_authenticated) (receive_confidential_authenticated #a);
   reveal_opaque (`%verify_and_decrypt_message) (verify_and_decrypt_message #a); // TODO: These reveals should be removeable.
-  match receive_confidential_authenticated #tag #a comm_keys_ids receiver msg_id tr with
+  match receive_confidential_authenticated #a comm_keys_ids receiver msg_id tr with
   | (None, tr_out) -> ()
   | (Some cm, tr_out) -> (
     let (Some msg_encrypted_signed, tr) = recv_msg msg_id tr in
-    let (Some sk_receiver, tr) = get_private_key receiver comm_keys_ids.private_keys (LongTermPkeKey comm_layer_pkenc_tag) tr in
+    let (Some sk_receiver, tr) = get_private_key receiver comm_keys_ids.private_keys (LongTermPkeKey (comm_layer_pkenc_tag a)) tr in
     let Some sender = get_sender msg_encrypted_signed in
-    let (Some vk_sender, tr) = get_public_key receiver comm_keys_ids.pki (LongTermSigKey comm_layer_sign_tag) sender tr in
-    verify_and_decrypt_message_proof #tag #invs.crypto_invs #a tr sender receiver msg_encrypted_signed sk_receiver vk_sender;
+    let (Some vk_sender, tr) = get_public_key receiver comm_keys_ids.pki (LongTermSigKey (comm_layer_sign_tag a)) sender tr in
+    verify_and_decrypt_message_proof #invs.crypto_invs #a tr sender receiver msg_encrypted_signed sk_receiver vk_sender;
     let Some cm = verify_and_decrypt_message #a receiver sk_receiver vk_sender msg_encrypted_signed in
-    let ((), tr) = trigger_event receiver (CommConfAuthReceiveMsg sender receiver (serialize a cm.payload)) tr in
-    assert(event_triggered tr receiver (CommConfAuthReceiveMsg sender receiver (serialize a cm.payload)));
+    let ((), tr) = trigger_event receiver (CommConfAuthReceiveMsg sender receiver cm.payload <: communication_core_event a) tr in
+    assert(event_triggered tr receiver (CommConfAuthReceiveMsg sender receiver cm.payload <: communication_core_event a));
     assert(trace_invariant tr);
     assert(tr == tr_out);
     ()
